polishing and documenting blake2.

src/Verse/CryptoLib/blake2/c/portable.v
@@ -7,18 +7,12 @@ Require Vector.
 Require Import Nat.
 Import VectorNotations.
 
+(** * Blake2 implementation in C
 
-(**
+This module provides the implementation of blake2 hashes in C. Both
+blake2b and blake2s implementations can be recovered from this module
+by passing the apporpriate config module [C : CONFIG].
 
-The blake2 implementation exposes both an iterator and a last block
-compressor. The iterator compresses in multiple of blocks and the last
-block compressor only handles the last < blocksize bytes. The last
-bock compressor assumes the following
-
-1. The buffer is of size at least the block length and
-
-2. Appropriate message padding has already been done and thus does not
-   bother to pad the date.
 
 *)
 
@@ -29,135 +23,140 @@ Module Blake2 (C : CONFIG).
   Definition Word : type direct  := word WORD_LOG_SIZE.
   Definition Hash  := Array HASH_SIZE  hostE Word.
   Definition Block := Array BLOCK_SIZE littleE Word.
+  Definition IV i (pf : i < 8) := Vector.nth_order IVVec pf.
 
+  (** Unlike the sha2 hashes, there is a difference in the structure
+      of blake2 in that there are special steps to be taken for the
+      last block. We leave out the padding issue for the last block
+      and expect the calling function to take care of this. Even
+      ignoring the padding, there are certain differences in the two.
 
-  (**
-      Type that captures a permutation of the message values. We
-      represent permutations by giving the vector of indices.
-   *)
-  Definition Perm := Vector.t {i | i < BLOCK_SIZE} BLOCK_SIZE.
+      - As opposed to a Merkel-Damgard hash like sha512, every block
+        needs the length of the message hashed sofar as its
+        argument. In the initial blocks, the lengths get updated by
+        the blocksize. However, the last block could be partial and
+        hence including this length in the compression should be done
+        carefully.
 
-    (** The round permutations of blake. Beyond round 10 it repeats the cycle. *)
+      - The last block also needs special finalisation flags. While,
+        these flags can be fixed when blake2 is run as a cryptographic
+        hash, the blake2 standard allows for other modes of operation
+        like message authentication and tree hashing which uses
+        different finalisation flags. Implementations here provide the
+        flexibility for tweaking these.
 
-    Definition RoundPerms : Vector.t Perm 10
-      := [
-          shuffleIndices [0 ;  1;  2;  3;  4;  5;  6;  7;  8;  9; 10; 11; 12; 13; 14; 15];
-	  shuffleIndices [14; 10;  4;  8;  9; 15; 13;  6;  1; 12;  0;  2; 11;  7;  5;  3];
-	  shuffleIndices [11;  8; 12;  0;  5;  2; 15; 13; 10; 14;  3;  6;  7;  1;  9;  4];
-	  shuffleIndices [7 ;  9;  3;  1; 13; 12; 11; 14;  2;  6;  5; 10;  4;  0; 15;  8];
-	  shuffleIndices [9 ;  0;  5;  7;  2;  4; 10; 15; 14;  1; 11; 12;  6;  8;  3; 13];
-	  shuffleIndices [2 ; 12;  6; 10;  0; 11;  8;  3;  4; 13;  7;  5; 15; 14;  1;  9];
-	  shuffleIndices [12;  5;  1; 15; 14; 13;  4; 10;  0;  7;  6;  3;  9;  2;  8; 11];
-	  shuffleIndices [13; 11;  7; 14; 12;  1;  3;  9;  5;  0; 15;  4;  8;  6;  2; 10];
-	  shuffleIndices [6 ; 15; 14;  9; 11;  3;  0;  8; 12;  2; 13;  7;  1;  4; 10;  5];
-	  shuffleIndices [10;  2;  8;  4;  7;  6;  1;  5; 15; 11;  9; 14;  3; 12; 13;  0]
-        ]%vector.
+      Due to the above reason, the module provides two functions, a
+      _blake2 iterator_, or _iterator_ for short that handles data in
+      multiples of blocks, and the _blake2 last block compressor_ or
+      _compressor_ for short which handles the last block of the
+      message.
 
-    Tactic Notation "crush_forall" tactic(tac)
-      := repeat match goal with
-                | [ |- Vector.Forall _  _  ] => constructor
-                | _ => tac
-                end.
+      We follow the standard idiom where the code for the iterator and
+      the last block compressor is wrapped into a section called
+      [Program].  *)
 
-    (** Let us prove that the round permutations are indeed permutations. *)
+  Section Program.
 
-    Theorem round_perms_are_permutations :  Vector.Forall (@Permutation BLOCK_SIZE) RoundPerms .
-      crush_forall (compute; crush_permutation_obligation 16).
-    Qed.
+    (** ** Program variables.
 
-    (** The blake2 implementation exposes both an iterator and a last
-        block compressor. The iterator compresses in multiple of
-        blocks and the last block compressor only handles the last <
-        blocksize bytes. The last bock compressor assumes the
-        following.
-
-        * The buffer is of size at least the block length, and
-
-        * Appropriate message padding has already been done and thus
-          does not bother to pad the date.
-
-        We follow the standard idiom for defining these two
-        functions. The two function has a slightly different set of
-        parameters and local register set. We use a single section for
-        both but distinguish there parameter and register list.
+      The program parameters and other variables become parameters to
+      the section of type [VariableT]. The iterator and the last block
+      compressor share a lot of program variables but there are indeed
+      variables that are relevant to one but not the other. We define
+      all these variables together in the same section. Since any coq
+      definition inside a section only has parameters that are
+      mentioned in the definiton, this works out well for use. The
+      only difference is that we need to be have two sets of
+      parameter, stack and register declaration in the code.
 
      *)
 
-    Section Program.
+    Variable progvar : VariableT.
+    Arguments progvar [k] _.
 
-      Variable progvar : VariableT.
-      Arguments progvar [k] _.
+    (** *** Parameters.
 
-      (** The G function. Takes 4 words which is either a row or
-          diagonal of the state and two message words. *)
+      The difference in the parameter list comes due to the following
+      reasons.
 
-      Definition G (a b c d m0 m1 : progvar Word) : code progvar :=
-        [ a ::=+ b; a ::=+ m0; d ::=^ a; d ::=>*> R0;
-          c ::=+ d;            b ::=^ c; b ::=>*> R1;
-          a ::=+ b; a ::=+ m1; d ::=^ a; d ::=>*> R2;
-          c ::=+ d;            b ::=^ c; b ::=>*> R3
-        ]%list.
+      - The iterator does not need to mention its message and the
+        count as these are implicitly supplied during the code
+        generation of an iterator, where as for the last block
+        compressor needs to define these explicitly.
 
-      (** * Parameters.
+      - The iterator is not done with the message yet, so it has a
+        responsibility to update the total count of bytes processed.
+        On the other hand the last block compressor only needs the
+        count of the bytes processed while compressing the last
+        block. Since there are no more blocks of message, it need not
+        update the count value. Due to the above difference, the
+        count, kept track of using two words, is passed as a reference
+        variable in iterator as opposed to normal variables in the
+        last block compressor.
 
-
-        The arguments taken by the function are the total bytes hashed
-        sofar and the hash sofar. The count of the data is kept in two
-        words. The iterator needs to update these count and hence
-        takes the arguments as reference variables whereas the last
-        block compressor takes.
-
-       *)
-
-      (** The array containing the last block. This is a parameter
-          only for the last block compressor as the iterator gets it
-          blocks implicitly.
-       *)
-
-      Variable LastBlock : progvar Block.
-      Variable NBytes    : progvar Word.
-
-      (** The reference variables that keeps track of the count of
-          bytes hashed. These counts are updated by the iterator and hence
-          needs to be reference variables
-       *)
-      Variable UpperRef LowerRef : progvar (Ref Word).
-
-      (** On the other hand the last block compressor does not need to
-          update any more as all uses of the count is already done. So
-          the variant here are ordinary variables.  *)
-      Variable Upper Lower : progvar Word.
-
-      (** The finalisation flags. These are only relevant for the last block *)
-      Variable f0 f1: progvar Word.
-      (** Finally the variable that contains the hash that is computed
-      so far. Both the iterator and the last block compressor needs
-      this parameter *)
-      Variable hash : progvar Hash.
+      - Finally the last block compressor needs finalisation constants
+        that need to be passed around which clearly the iterator does
+        not need
 
 
-      Definition paramIterator  : Declaration
-        := [Var UpperRef; Var LowerRef; Var hash].
-      Definition paramLastBlock : Declaration
-        := [Var LastBlock; Var NBytes; Var Upper; Var Lower; Var f0; Var f1; Var hash].
+      To summarise we have the following
 
-      Variable h0 h1 h2 h3 h4 h5 h6 h7 : progvar Word.
-      Definition H  : VarIndex progvar 8 Word := varIndex [h0; h1; h2; h3; h4; h5; h6; h7].
-      Definition stack : Declaration := Vector.map Var [h0 ;h1 ;h2; h3; h4; h5; h6; h7].
+       - The reference variables [UpperRef], and [LowerRef] that is
+         unique to to the iterator,
 
-      (** Register cache for the current block *)
-      Variable w0 w1 w2 w3 w4 w5 w6 w7 w8 w9 w10 w11 w12 w13 w14 w15 : progvar Word.
+       - The variables [LastBlock], [NBytes], [Upper] [Lower], [f0]
+         and [f1] unique to the last block iterator, and
 
-      Definition message_variables
+       - The variable [hash] which is common to both.
+
+     *)
+
+
+
+    Variable UpperRef LowerRef : progvar (Ref Word).
+
+    Variable LastBlock : progvar Block.
+    Variable NBytes    : progvar Word.
+    Variable Upper Lower : progvar Word.
+    Variable f0 f1: progvar Word.
+
+    Variable hash : progvar Hash.
+
+
+    Definition paramIterator  : Declaration
+      := [Var UpperRef; Var LowerRef; Var hash].
+    Definition paramLastBlock : Declaration
+      := [Var LastBlock; Var NBytes; Var Upper; Var Lower; Var f0; Var f1; Var hash].
+
+    (** *** The stack variables.
+
+        The iterator also keeps a copy of the hash in local variables
+        to speed up access. On register rich machines this could
+        potentially end up on actual registers and hence could become
+        fast.
+
+     *)
+    Variable h0 h1 h2 h3 h4 h5 h6 h7 : progvar Word.
+    Definition stack : Declaration := Vector.map Var [h0 ;h1 ;h2; h3; h4; h5; h6; h7].
+    Definition H  : VarIndex progvar 8 Word := varIndex [h0; h1; h2; h3; h4; h5; h6; h7].
+
+    (** *** The register variables.
+
+        We start with a register cache for the message block.
+
+     *)
+    Variable w0 w1 w2 w3 w4 w5 w6 w7 w8 w9 w10 w11 w12 w13 w14 w15 : progvar Word.
+
+    Definition message_variables
       := [w0; w1; w2; w3; w4; w5; w6; w7; w8; w9; w10; w11; w12; w13; w14; w15].
 
-      Definition W : VarIndex progvar BLOCK_SIZE Word := varIndex message_variables.
 
 
-    (** * The state variables
+    (** *** The state variables
 
         The state of the hashing function is a 4x4 matrix of
-        words. The rounds transform this state using the [G] function.
+        words. The rounds transform this state using the [G] functions
+        applied to either the rows or the diagonals of this matrix.
 
      *)
     Variable v0 v4 v8  v12
@@ -171,27 +170,60 @@ Module Blake2 (C : CONFIG).
                           v3 ; v7 ; v11 ; v15
                         ].
 
-    (** The iterator needs registers U, L which together keep track of
-       the total bytes hashed so far. In the case of the last block iterator, we reuse
-       the parameters Upper and Lower and do not need them
+    (** *** Registers to manage byte count.
+
+        Recall that each of the blake2 blocks is compressed using a
+        compression function that makes use of the length of the
+        message as auxiliary input. The message length is kept track
+        of as a set of two words and hence we need to explicitly do
+        arithmetic in twice the precision. In the iterator this byte
+        count is kept in the reference variables [UpperRef] and
+        [LowerRef] where as in the last block compressor it is merely
+        passed as parameters [Upper] and [Lower]. As a result these
+        functions have the following additional register variables.
+
+        - The [C] and the [LMSB] registers used to perform the count
+          update with twice the precision. The variable [C] is used to
+          compute the carry generated when the lower words are added
+          and the [LMSB] is used as an intermediate register to hold
+          the most significant bit of the lower portion of the count.
+
+        - The iterator also define two variables [U] and [V] that is
+          to be used instead of the reference variables [UpperRef] and
+          [LowerRef].
+
+
      *)
 
+    Variable C LMSB : progvar Word.
     Variable U L    : progvar Word.
 
-    (** While updating the count, we need to keep track of the carry
-        from the lower word to the higher word and these variables are
-        used for that purpose. They are required by both the iterator
-        and their last block compressor *)
+    Definition regLastBlock
+      := Vector.map Var (Vector.append (Vector.append message_variables state) [C ; LMSB]).
 
-    Variable C LMSB : progvar Word.
-
-    Definition commonRegs := Vector.append message_variables state.
     Definition regIterator : Declaration
-      := Vector.map Var (Vector.append commonRegs [ U   ; L   ; C ; LMSB])%vector.
-    Definition regLastBlock : Declaration :=
-      Vector.map Var (Vector.append commonRegs [ C ; LMSB]).
+      := Vector.append regLastBlock  (Vector.map Var [ U   ; L])%vector.
 
-    (** Code to update the count of bytes *)
+
+    (** ** Updating the count.
+
+        The main idea is to compute the carry arising while adding the
+        lower word.
+
+        - Compute the carry occurring on most significant bit by
+          masking off the MSB and performing the addition. Shift it to
+          the least significant bit.
+
+        - Compute the MSB of the lower word and shift it to the least
+          significant bit.
+
+        - Add the previous two carries to obtain the carry occurring
+          on the MSB of the lower word in bit position 2.
+
+        - Shift it right once more to obtain the actual carry.
+
+     *)
+
     Section UpdateCount.
 
       Hint Resolve NPeano.Nat.add_pos_pos.
@@ -202,18 +234,26 @@ Module Blake2 (C : CONFIG).
       Qed.
       Hint Resolve zeroLtPower2.
 
-      (** This mask is used to mask out the top most bit for computing the carry *)
+      (** This constant used to mask out the top most bit for
+          computing the carry
+       *)
       Definition mask : constant Word.
         refine (let allones := Vector.const xF (2*2^WORD_LOG_SIZE) in
                 @Vector.replace_order _ _ allones 0 _ x7); simpl.
         eauto.
       Defined.
-      (** Block size now as a program constant *)
-      Definition bsize : constant Word := fromNat (BLOCK_SIZE * size Word).
+
+
+      (* To make the update count work uniformly both for the iterator
+         as well as the last block compressor, we need to parameterise
+         over both the upper and lower arguments and also the size
+         argument.
+       *)
 
       Variable A : Type.
       Variable a_is_rarg : RARG progvar direct Word A.
       Variable byteCount : A.
+
       Definition UPDATE_COUNTER (u l : progvar Word) : code progvar :=
         [ (* We first ensure that the variable C gets the carry that overflows
              when l is added bsize. For this we first need to get the msb of l
@@ -240,20 +280,94 @@ Module Blake2 (C : CONFIG).
     End UpdateCount.
 
     Arguments UPDATE_COUNTER [A a_is_rarg] _ _ _ .
-    Definition UPDATE := UPDATE_COUNTER bsize U L.
-    Definition UPDATE_LAST := UPDATE_COUNTER NBytes U L.
+
+    (** The update count function as defined for the iterator and the
+        last block compressor respectively *)
+    Definition UPDATE_COUNTER_ITER :=
+      let bsize : constant Word := fromNat (BLOCK_SIZE * size Word)
+      in UPDATE_COUNTER bsize U L.
+
+    Definition UPDATE_COUNTER_LAST := UPDATE_COUNTER NBytes Upper Lower.
+
+    (** ** The blake round function.
+
+
+      A single round of blake function consists of performing the G
+      function, first on the rows and then on the diagonals of the
+      state matrix. The message words that are used change merely
+      permuted and then used respectively.
+
+     *)
+
+    (** *** The G function.
+
+        The G function defined below takes 4 words which constitute
+        either a row or a diagonal of the state matrix. In addition it
+        takes two message words
+
+     *)
+
+    Definition G (a b c d m0 m1 : progvar Word) : code progvar :=
+      [
+        a ::=+ b; a ::=+ m0; d ::=^ a; d ::=>*> R0;
+        c ::=+ d;            b ::=^ c; b ::=>*> R1;
+        a ::=+ b; a ::=+ m1; d ::=^ a; d ::=>*> R2;
+        c ::=+ d;            b ::=^ c; b ::=>*> R3
+      ]%list.
+
+    (** *** Message permutations.
+
+       Each round uses the entire set of the message word but
+       in different order captured by a message permutations
+
+     *)
+
+    Definition Perm := Vector.t {i | i < BLOCK_SIZE} BLOCK_SIZE.
+    Definition RoundPerms : Vector.t Perm 10
+      := [
+          shuffleIndices [0 ;  1;  2;  3;  4;  5;  6;  7;  8;  9; 10; 11; 12; 13; 14; 15];
+	  shuffleIndices [14; 10;  4;  8;  9; 15; 13;  6;  1; 12;  0;  2; 11;  7;  5;  3];
+	  shuffleIndices [11;  8; 12;  0;  5;  2; 15; 13; 10; 14;  3;  6;  7;  1;  9;  4];
+	  shuffleIndices [7 ;  9;  3;  1; 13; 12; 11; 14;  2;  6;  5; 10;  4;  0; 15;  8];
+	  shuffleIndices [9 ;  0;  5;  7;  2;  4; 10; 15; 14;  1; 11; 12;  6;  8;  3; 13];
+	  shuffleIndices [2 ; 12;  6; 10;  0; 11;  8;  3;  4; 13;  7;  5; 15; 14;  1;  9];
+	  shuffleIndices [12;  5;  1; 15; 14; 13;  4; 10;  0;  7;  6;  3;  9;  2;  8; 11];
+	  shuffleIndices [13; 11;  7; 14; 12;  1;  3;  9;  5;  0; 15;  4;  8;  6;  2; 10];
+	  shuffleIndices [6 ; 15; 14;  9; 11;  3;  0;  8; 12;  2; 13;  7;  1;  4; 10;  5];
+          shuffleIndices [10;  2;  8;  4;  7;  6;  1;  5; 15; 11;  9; 14;  3; 12; 13;  0]
+        ]%vector.
+
+    (** Let us digress a bit and prove that the above shuffles are
+        indeed permutations.  *)
+    Tactic Notation "crush_forall" tactic(tac)
+      := repeat match goal with
+                | [ |- Vector.Forall _  _  ] => constructor
+                | _ => tac
+                end.
+
+    Theorem round_perms_are_permutations :  Vector.Forall (@Permutation BLOCK_SIZE) RoundPerms .
+      crush_forall (compute; crush_permutation_obligation 16).
+    Qed.
+
+    (** *** The round function.
+
+         We now give the blake round function as a section
+         parameterised by the round number.
+
+     *)
 
     Section Round.
-      Variable r : nat. (** Round number *)
+
+      Variable r : nat.
       Variable rBondPf : r < ROUNDS.
 
-      Print Vector.nth_order.
+      (** The register cache corresponding to the permuted message *)
       Definition M : VarIndex progvar BLOCK_SIZE Word.
-        verse( varIndex (select message_variables
+        verse (varIndex (select message_variables
                                 (@Vector.nth_order _ _ RoundPerms (r mod 10) _))).
       Defined.
 
-      Definition round : code progvar.
+      Definition ROUND : code progvar.
         verse (G v0 v4 v8  v12 (M 0 _) (M 1 _) ++
                G v1 v5 v9  v13 (M 2 _) (M 3 _) ++
                G v2 v6 v10 v14 (M 4 _) (M 5 _) ++
@@ -266,16 +380,22 @@ Module Blake2 (C : CONFIG).
       Defined.
     End Round.
 
-    Definition ALL_ROUNDS := iterate round.
+    (** The entire set of rounds *)
+    Definition ALL_ROUNDS := iterate ROUND.
 
-    (** We are now ready to define both the iterator and the last block compressor *)
 
     Definition SETUP : code progvar.
       verse ( [ U ::== UpperRef[- 0 -]; L ::== LowerRef[- 0 -] ] ++ loadCache hash H ).
     Defined.
 
-    Definition IV i (pf : i < 8) := Vector.nth_order IVVec pf.
+    (** ** The initialisation of state.
 
+        The initialisation uses the previous hash values and the
+        iv. Depending on whether the initialisation for a block in
+        between or the last block there is a slight difference in the
+        initialisation code.
+
+     *)
     Definition INIT_STATE : code progvar.
       verse
         [ v0 ::== h0;
@@ -297,7 +417,6 @@ Module Blake2 (C : CONFIG).
         ]%list.
     Defined.
 
-
     Definition INIT_STATE_LAST : code progvar.
       verse
         [ v0 ::== h0;
@@ -312,14 +431,21 @@ Module Blake2 (C : CONFIG).
 	  v9  ::== IV 1 _;
 	  v10 ::== IV 2 _;
 	  v11 ::== IV 3 _;
-	  v12 ::= IV 4 _ [^] L;
-	  v13 ::= IV 5 _ [^] U;
+	  v12 ::= IV 4 _ [^] Lower;
+	  v13 ::= IV 5 _ [^] Upper;
 	  v14 ::= IV 6 _ [^] f0;
 	  v15 ::= IV 7 _ [^] f1
         ]%list.
       Defined.
 
 
+    (** ** Load message into register cache.
+
+        To speed up the hashing we load the message into the register
+        cache W.
+
+     *)
+    Definition W : VarIndex progvar BLOCK_SIZE Word := varIndex message_variables.
     Definition LOAD_MESSAGE_I (blk : progvar Block) (i : nat) (pf : i < BLOCK_SIZE)
       : code progvar.
       verse [ W i _ ::== blk [- i -] ]%list.
@@ -328,6 +454,11 @@ Module Blake2 (C : CONFIG).
       := foreach (indices blk) (LOAD_MESSAGE_I blk).
 
 
+    (** ** Updating the hash.
+
+        After performing the rounds of blake, the hash gets updated as follows.
+
+     *)
     Definition UPDATE_HASH : code progvar :=
       [ h0 ::=^ v0 ; h0 ::=^ v8;
         h1 ::=^ v1 ; h0 ::=^ v9;
@@ -339,29 +470,31 @@ Module Blake2 (C : CONFIG).
         h7 ::=^ v7 ; h0 ::=^ v15
       ]%list.
 
+    (** In the iterator one needs to update the hash array as well as
+        the reference variables UpperRef and LowerRef.  *)
     Definition FINALISE : code progvar.
       verse ([ MOVE U TO UpperRef[- 0 -]; MOVE L TO LowerRef[- 0 -] ] ++ moveBackCache hash H ).
     Defined.
 
-    Definition Iterator : iterator Block progvar :=
-      {| setup := SETUP;
-         process := fun blk => UPDATE
-                              ++ INIT_STATE
-                              ++ LOAD_MESSAGE blk
-                              ++ ALL_ROUNDS
-                              ++ UPDATE_HASH;
 
+    Definition PROCESS_BLOCK blk :=
+      LOAD_MESSAGE blk
+      ++ ALL_ROUNDS
+      ++ UPDATE_HASH.
+
+    (** ** The BLAKE2 iterator and the last block compressor.  *)
+    Definition Iterator : iterator Block progvar :=
+      {| setup   := SETUP;
+         process := fun blk => UPDATE_COUNTER_ITER ++ INIT_STATE ++ PROCESS_BLOCK blk;
          finalise := FINALISE
       |}.
 
     Definition LastBlockCompress :=
       loadCache hash H
-                ++ UPDATE_LAST
-                ++ INIT_STATE
-                ++ LOAD_MESSAGE LastBlock
-                ++ ALL_ROUNDS
+                ++ UPDATE_COUNTER_LAST
+                ++ INIT_STATE_LAST
+                ++ PROCESS_BLOCK  LastBlock
                 ++ moveBackCache hash H.
+    End Program.
 
-
-  End  Program.
 End Blake2.
